coq/examples/reduction_gen.v
@@ -1,0 +1,18 @@
+From Coq Require Import ZArith List String.
+Import ListNotations.
+Require Import MIRSyntax MIRSemantics.
+
+Module M := MIR.
+Module MS := MIRSemantics.
+
+Module Reduction_gen.
+
+Definition prog : list M.stmt :=
+  [ M.SStoreShared (M.EPtrAdd (M.EVar "_1") (M.EVar "_6)")) (M.EVar "_3") M.TyF32;
+    M.SBarrierShared;
+    M.SFor "_loop_counter" 3 [ M.SLoadShared "_18" (M.EPtrAdd (M.EVar "_1") (M.EVar "_20)")) M.TyF32;
+        M.SLoadShared "_21" (M.EPtrAdd (M.EVar "_1") (M.EVar "_23)")) M.TyF32;
+        M.SStoreShared (M.EPtrAdd (M.EVar "_1") (M.EVar "_27)")) (M.EAdd (M.EVar "_18") (M.EVar "_21")) M.TyF32;
+        M.SBarrierShared ] ].
+
+End Reduction_gen.
